RefineMonadicVCG.thy
@@ -37,6 +37,9 @@ lemma Some_le_mm3_Some_conv[vcg_simp_rules]: "Some t \<le> mm3 t' (Some t'') \<l
 lemma Some_le_emb'_conv[vcg_simp_rules]: "Some t \<le> emb' Q ft x \<longleftrightarrow> Q x \<and> t \<le> ft x"
   by (auto simp: emb'_def)
 
+lemma Some_eq_emb'_conv: "emb' Q tf s = Some t \<longleftrightarrow> (Q s \<and> t = tf s)"
+  unfolding emb'_def by(auto split: if_splits)
+
 
 lemma not_cons_is_Nil_conv[simp]: "(\<forall>y ys. l \<noteq> y # ys) \<longleftrightarrow> l=[]" by (cases l) auto
 
